cedar-lean/Cedar/Thm/Data/Control.lean
@@ -57,7 +57,96 @@ theorem do_error {res : Except ε α} {e : ε} {f : α → β} :
   res = .error e
 := by cases res <;> simp
 
-theorem do_ok {res : Except ε α} {f : α → β} :
+theorem do_ok_eq_ok {res : Except ε α} {f : α → β} :
   (do let v ← res ; .ok (f v)) = .ok b ↔
   ∃ a, res = .ok a ∧ f a = b
 := by cases res <;> simp
+
+theorem do_eq_ok {res : Except ε α} {f : α → Except ε β} :
+  (do let v ← res ; f v) = .ok b ↔
+  ∃ a, res = .ok a ∧ f a = .ok b
+:= by cases res <;> simp
+
+theorem do_eq_ok₂ {res₁ res₂: Except ε PUnit} :
+  (do res₁ ; res₂) = .ok () → res₁ = .ok () ∧ res₂ = .ok ()
+:= by
+  cases res₁ <;> cases res₂ <;> simp
+
+theorem to_option_some {v : α} {res: Except ε α} :
+  res.toOption = .some v ↔ res = .ok v
+:= by
+  constructor
+  case mp =>
+    intro h
+    simp [Except.toOption] at h
+    split at h <;> simp at h
+    subst h
+    rfl
+  case mpr =>
+    intro h
+    simp only [Except.toOption, h]
+
+theorem to_option_none {res: Except ε α} :
+  res.toOption = .none → (∃ err, res = .error err)
+:= by
+  intro h
+  simp [Except.toOption] at h
+  split at h <;> simp at h
+  rename_i err
+  exists err
+
+theorem to_option_left_ok {α ε₁ ε₂} {v : α} {res₁ : Except ε₁ α} {res₂ : Except ε₂ α} :
+  res₁.toOption = res₂.toOption → res₁ = .ok v → res₂ = .ok v
+:= by
+  intro h₀ h₁
+  simp [Except.toOption] at h₀
+  repeat split at h₀
+  · simp only [Except.ok.injEq]
+    simp only [Option.some.injEq] at h₀
+    simp only [Except.ok.injEq] at h₁
+    simp only [← h₀]; exact h₁
+  · cases h₀
+  · cases h₁
+
+theorem to_option_right_ok {α ε₁ ε₂} {v : α} {res₁ : Except ε₁ α} {res₂ : Except ε₂ α} :
+  res₁.toOption = res₂.toOption → res₂ = .ok v → res₁ = .ok v
+:= by
+  intro h
+  symm at h
+  exact to_option_left_ok h
+
+theorem to_option_right_ok' {α ε₁ ε₂} {v : α} {res₁ : Except ε₁ α} :
+  res₁.toOption = ((.ok v) : Except ε₂ α).toOption → res₁ = Except.ok v
+:= by
+  generalize h : ((.ok v) : Except ε₂ α) = res₂
+  symm at h
+  intro h₁
+  exact to_option_right_ok h₁ h
+
+theorem to_option_left_ok' {α ε₁ ε₂} {v : α} {res₂ : Except ε₂ α} :
+  ((.ok v) : Except ε₁ α).toOption = res₂.toOption → res₂ = Except.ok v
+:= by
+  intro h
+  symm at h
+  exact to_option_right_ok' h
+
+theorem to_option_left_err {ε₁ ε₂ α} {err₁: ε₁} {res₂ : Except ε₂ α} :
+  (Except.error err₁).toOption = res₂.toOption → ∃ err₂, res₂ = .error err₂
+:= by
+  intro h
+  simp [Except.toOption] at h
+  repeat split at h
+  · cases h
+  · simp only [Except.error.injEq, exists_eq']
+
+theorem to_option_right_err {ε₂ ε₁ α} {err₂: ε₂} {res₁ : Except ε₁ α} :
+  res₁.toOption = (Except.error err₂).toOption → ∃ err₁, res₁ = .error err₁
+:= by
+  intro h
+  symm at h
+  exact to_option_left_err h
+
+theorem do_error_to_option {res : Except ε α} {e : ε} :
+  (do let (_ : α) ← res ; (.error e : Except ε α)).toOption = .none
+:= by
+  cases res <;> simp [Except.toOption]
