cedar-lean/Cedar/Thm/TPE.lean
@@ -1,0 +1,150 @@
+/-
+ Copyright Cedar Contributors
+
+ Licensed under the Apache License, Version 2.0 (the "License");
+ you may not use this file except in compliance with the License.
+ You may obtain a copy of the License at
+
+      https://www.apache.org/licenses/LICENSE-2.0
+
+ Unless required by applicable law or agreed to in writing, software
+ distributed under the License is distributed on an "AS IS" BASIS,
+ WITHOUT WARRANTIES OR CONDITIONS OF ANY KIND, either express or implied.
+ See the License for the specific language governing permissions and
+ limitations under the License.
+-/
+
+import Cedar.TPE
+import Cedar.Spec
+import Cedar.Validation
+import Cedar.Thm.TPE.Input
+import Cedar.Thm.TPE.Soundness
+import Cedar.Thm.Validation
+
+/-!
+This file defines the main theorem of TPE soundness and its associated lemmas.
+-/
+
+namespace Cedar.Thm
+
+open Cedar.TPE
+open Cedar.Spec
+open Cedar.Validation
+open Cedar.Thm
+
+/-- The main lemma: Evaluating a residual derived from partially evaluating
+a well-typed expression is equivalent to that of evaluating the original
+expression, provided that requests and entities are consistent. The equivalency
+is defined using `Except.toOption`.
+-/
+theorem partial_evaluate_is_sound
+  {x : TypedExpr}
+  {req : Request}
+  {es : Entities}
+  {preq : PartialRequest}
+  {pes : PartialEntities}
+  {env : Environment} :
+  TypedExpr.WellTyped env x →
+  RequestAndEntitiesMatchEnvironment env req es →
+  RequestAndEntitiesRefine req es preq pes →
+  (Spec.evaluate x.toExpr req es).toOption = (Residual.evaluate (Cedar.TPE.evaluate x preq pes) req es).toOption
+:= by
+  intro h₁ h₂ h₃
+  induction h₁
+  case lit =>
+    exact partial_evaluate_is_sound_lit
+  case var =>
+    exact partial_evaluate_is_sound_var h₃
+  case ite x₁ x₂ x₃ hwt _ _ hₜ _ hᵢ₁ hᵢ₂ hᵢ₃ =>
+    exact partial_evaluate_is_sound_ite h₂ hwt hₜ hᵢ₁ hᵢ₂ hᵢ₃
+  case and x₁ x₂ hᵢ₁ hᵢ₂ hᵢ₃ hᵢ₄ hᵢ₅ hᵢ₆ =>
+    exact partial_evaluate_is_sound_and h₂ hᵢ₁ hᵢ₂ hᵢ₃ hᵢ₄ hᵢ₅ hᵢ₆
+  case or x₁ x₂ hᵢ₁ hᵢ₂ hᵢ₃ hᵢ₄ hᵢ₅ hᵢ₆ =>
+    exact partial_evaluate_is_sound_or h₂ hᵢ₁ hᵢ₂ hᵢ₃ hᵢ₄ hᵢ₅ hᵢ₆
+  case unaryApp op₁ x₁ ty hᵢ₁ =>
+    exact partial_evaluate_is_sound_unary_app hᵢ₁
+  case binaryApp op₂ x₁ x₂ ty _ hwt howt hᵢ₁ hᵢ₂ =>
+    exact partial_evaluate_is_sound_binary_app h₂ h₃ hwt howt hᵢ₁ hᵢ₂
+  case hasAttr_entity ety x₁ attr hᵢ₁ =>
+    exact partial_evaluate_is_sound_has_attr h₃ hᵢ₁
+  case hasAttr_record rty x₁ attr hᵢ₁ =>
+    exact partial_evaluate_is_sound_has_attr h₃ hᵢ₁
+  case getAttr_entity ety rty x₁ attr ty hᵢ₁ =>
+    exact partial_evaluate_is_sound_get_attr h₃ hᵢ₁
+  case getAttr_record rty x₁ attr ty hᵢ₁ =>
+    exact partial_evaluate_is_sound_get_attr h₃ hᵢ₁
+  case set ls ty hᵢ₁ =>
+    exact partial_evaluate_is_sound_set hᵢ₁
+  case record rty m hᵢ₁ hᵢ₁ =>
+    exact partial_evaluate_is_sound_record hᵢ₁
+  case call xfn args ty hᵢ₁ =>
+    exact partial_evaluate_is_sound_call hᵢ₁
+
+/-- The main theorem of TPE: Evaluating a result residual is equivalent to
+evaluating the input policy, given valid and consistent requests and entities.
+The equivalence is w.r.t authorization results. That is, the evaluation results
+are strictly equal when they are `.ok` or both errors (captured by
+`Except.toOption`). We do not care if the error types match because they do not
+impact authorization results. As a matter of fact, they do not match because all
+errors encountered during TPE are represented by an `error` residual, whose
+interpretation always produces an `extensionError`.
+-/
+theorem partial_evaluate_policy_is_sound
+  {schema : Schema}
+  {residual : Residual}
+  {policy : Policy}
+  {req : Request}
+  {es : Entities}
+  {preq : PartialRequest}
+  {pes : PartialEntities} :
+  evaluatePolicy schema policy preq pes = .ok residual   →
+  isValidAndConsistent schema req es preq pes = .ok () →
+  (Spec.evaluate policy.toExpr req es).toOption = (Residual.evaluate residual req es).toOption
+:= by
+  intro h₁ h₂
+  have h₃ := consistent_checks_ensure_refinement h₂
+  simp [evaluatePolicy] at h₁
+  split at h₁ <;> try cases h₁
+  split at h₁ <;> try cases h₁
+  simp [do_ok_eq_ok] at h₁
+  rcases h₁ with ⟨_, ⟨_, h₁₁⟩, h₁₂⟩
+  simp [Except.mapError] at h₁₁
+  split at h₁₁ <;> try cases h₁₁
+  rename_i env heq₁ _ ty _ _ heq₂
+  simp [isValidAndConsistent] at h₂
+  split at h₂ <;> try cases h₂
+  rename_i heq₃
+  simp [heq₁] at heq₃
+  subst heq₃
+  have ⟨h₂₁, h₂₂⟩ := do_eq_ok₂ h₂
+  simp only [isValidAndConsistent.requestIsConsistent, Bool.or_eq_true, Bool.not_eq_eq_eq_not,
+    Bool.not_true, Bool.and_eq_true, decide_eq_true_eq] at h₂₁
+  split at h₂₁ <;> try cases h₂₁
+  rename_i heq₃
+  simp only [not_or, Bool.not_eq_false] at heq₃
+  rcases heq₃ with ⟨_, heq₃⟩
+  simp only [isValidAndConsistent.entitiesIsConsistent, Bool.or_eq_true, Bool.not_eq_eq_eq_not,
+    Bool.not_true] at h₂₂
+  split at h₂₂ <;> try cases h₂₂
+  rename_i heq₄
+  simp only [not_or, Bool.not_eq_false] at heq₄
+  rcases heq₄ with ⟨_, heq₄⟩
+  simp [Except.isOk, Except.toBool] at heq₄
+  split at heq₄ <;> cases heq₄
+  rename_i heq₄
+  have h₄ := request_and_entities_match_env heq₃ heq₄
+  have h₅ := typechecked_is_well_typed_after_lifting h₄ heq₂
+  have h₆ := partial_evaluate_is_sound h₅ h₄ h₃
+  subst h₁₂
+  have h₇ := type_of_preserves_evaluation_results (empty_capabilities_invariant req es) h₄ heq₂
+  have h₈ : Spec.evaluate (substituteAction env.reqty.action policy.toExpr) req es = Spec.evaluate policy.toExpr req es := by
+    simp [RequestAndEntitiesMatchEnvironment] at h₄
+    rcases h₄ with ⟨h₄, _⟩
+    simp [InstanceOfRequestType] at h₄
+    rcases h₄ with ⟨_, h₄, _⟩
+    rw [←h₄]
+    exact substitute_action_preserves_evaluation policy.toExpr req es
+  simp [h₈] at h₇
+  rw [h₇, type_lifting_preserves_expr]
+  exact h₆
+end Cedar.Thm
