cedar-lean/Cedar/Thm/TPE/Input.lean
@@ -1,0 +1,119 @@
+/-
+ Copyright Cedar Contributors
+
+ Licensed under the Apache License, Version 2.0 (the "License");
+ you may not use this file except in compliance with the License.
+ You may obtain a copy of the License at
+
+      https://www.apache.org/licenses/LICENSE-2.0
+
+ Unless required by applicable law or agreed to in writing, software
+ distributed under the License is distributed on an "AS IS" BASIS,
+ WITHOUT WARRANTIES OR CONDITIONS OF ANY KIND, either express or implied.
+ See the License for the specific language governing permissions and
+ limitations under the License.
+-/
+
+import Cedar.TPE.Input
+import Cedar.Spec
+import Cedar.Validation
+import Cedar.Thm.Validation
+
+/-!
+This file defines theorems related to the inputs of TPE.
+-/
+
+namespace Cedar.Thm
+
+open Cedar.TPE
+open Cedar.Spec
+open Cedar.Validation
+open Cedar.Thm
+
+theorem decide_eq_implies_eq {α} [DecidableEq α] {y : α} :
+  ∀ x, decide (x = y) → x = y := by
+      simp only [decide_eq_true_eq, imp_self, implies_true]
+
+inductive PartialIsValid {α} : (α → Prop) → Option α -> Prop
+  | some (p : α → Prop) (x : α)
+    (h : p x) :
+    PartialIsValid p (.some x)
+  | none :
+    PartialIsValid p .none
+
+theorem partial_is_valid_rfl (f : α → Bool) (p : α → Prop) (o : Option α) :
+  (∀ x, f x = true → p x) → partialIsValid o f → PartialIsValid p o
+:= by
+  intro h₁
+  simp [partialIsValid, Option.map]
+  split <;> simp [Option.getD]
+  case _ x =>
+    intro h₂
+    constructor
+    exact h₁ x h₂
+  case _ =>
+    constructor
+
+def RequestRefines (req : Request) (preq : PartialRequest) : Prop :=
+  PartialIsValid (· = req.principal) preq.principal.asEntityUID ∧
+  req.action = preq.action ∧
+  PartialIsValid (· = req.resource) preq.resource.asEntityUID  ∧
+  PartialIsValid (· = req.context) preq.context
+
+def EntitiesRefine (es : Entities) (pes : PartialEntities) : Prop :=
+   ∀ a e₂, pes.find? a = some e₂ → (∃ e₁, es.find? a = some e₁ ∧
+    PartialIsValid (· = e₁.attrs) e₂.attrs ∧
+    PartialIsValid (· = e₁.ancestors) e₂.ancestors  ∧
+    PartialIsValid (· = e₁.tags) e₂.tags)
+
+/-- Concrete request `req` and entities `es` refine their partial counterparts
+`peq` and `pes`.
+-/
+def RequestAndEntitiesRefine (req : Request) (es : Entities) (preq : PartialRequest) (pes : PartialEntities) : Prop :=
+  RequestRefines req preq ∧ EntitiesRefine es pes
+
+/-- Requests and entities that pass `isValidAndConsistent` satisfy `RequestAndEntitiesRefine`.
+-/
+theorem consistent_checks_ensure_refinement {schema : Schema} {req : Request} {es : Entities} {preq : PartialRequest} {pes : PartialEntities} :
+  isValidAndConsistent schema req es preq pes = .ok () → RequestAndEntitiesRefine req es preq pes
+:= by
+  intro h
+  simp [isValidAndConsistent] at h
+  split at h <;> try cases h
+  rcases do_eq_ok₂ h with ⟨h₁, h₂⟩
+  simp [RequestAndEntitiesRefine]
+  constructor
+  case _ =>
+    simp [RequestRefines]
+    simp [isValidAndConsistent.requestIsConsistent] at h₁
+    split at h₁ <;> simp at h₁
+    rcases h₁ with ⟨h₁₁, h₁₂, h₁₃, h₁₄⟩
+    constructor
+    exact partial_is_valid_rfl (fun x => decide (x = req.principal)) (fun x => x = req.principal) preq.principal.asEntityUID decide_eq_implies_eq h₁₁
+    constructor
+    exact h₁₂
+    constructor
+    exact partial_is_valid_rfl (fun x => decide (x = req.resource)) (fun x => x = req.resource) preq.resource.asEntityUID decide_eq_implies_eq h₁₃
+    exact partial_is_valid_rfl (fun x => decide (x = req.context)) (fun x => x = req.context) preq.context decide_eq_implies_eq h₁₄
+  case _ =>
+    simp [isValidAndConsistent.entitiesIsConsistent] at h₂
+    split at h₂ <;> simp at h₂
+    simp [isValidAndConsistent.entitiesMatch] at h₂
+    simp [EntitiesRefine]
+    intro uid data₂ hᵢ
+    replace hᵢ := Data.Map.find?_mem_toList hᵢ
+    simp [Data.Map.toList] at hᵢ
+    specialize h₂ uid data₂ hᵢ
+    split at h₂ <;> simp at h₂
+    rcases h₂ with ⟨⟨h₂₁, h₂₂⟩, h₂₃⟩
+    rename_i data₁ heq
+    exists data₁
+    constructor
+    exact heq
+    constructor
+    exact partial_is_valid_rfl (fun x => decide (x = data₁.attrs)) (fun x => x = data₁.attrs) data₂.attrs decide_eq_implies_eq h₂₁
+    constructor
+    exact partial_is_valid_rfl (fun x => decide (x = data₁.ancestors)) (fun x => x = data₁.ancestors) data₂.ancestors decide_eq_implies_eq h₂₂
+    exact partial_is_valid_rfl (fun x => decide (x = data₁.tags)) (fun x => x = data₁.tags) data₂.tags decide_eq_implies_eq h₂₃
+
+end Cedar.Thm
