cedar-lean/Cedar/Thm/Validation/Typechecker.lean
@@ -98,3 +98,345 @@ theorem type_of_is_sound {e : Expr} {c₁ c₂ : Capabilities} {env : Environmen
       exact @type_of_is_sound xᵢ
     exact type_of_call_is_sound h₁ h₂ h₃ ih
 termination_by sizeOf e
+
+/-- The type checker, if succeeds, should produce a typed expression that
+evaluates to the same result as the input expression.
+-/
+theorem type_of_preserves_evaluation_results {e : Expr} {c₁ c₂ : Capabilities} {env : Environment} {ty : TypedExpr} {request : Request} {entities : Entities} :
+  CapabilitiesInvariant c₁ request entities →
+  RequestAndEntitiesMatchEnvironment env request entities →
+  typeOf e c₁ env = .ok (ty, c₂) →
+  evaluate e request entities = evaluate ty.toExpr request entities
+:= by
+  intro h₁ h₂ h₃
+  induction e, c₁, env using typeOf.induct generalizing ty c₂
+  case _ =>
+    simp [typeOf, typeOfLit, ok] at h₃
+    split at h₃ <;>
+    try (
+      simp at h₃
+      rcases h₃ with ⟨h₃, _⟩
+      subst h₃
+      simp only [TypedExpr.toExpr]
+    )
+    split at h₃ <;> simp [err] at h₃
+    rcases h₃ with ⟨h₃, _⟩
+    subst h₃
+    simp only [TypedExpr.toExpr]
+  case _ =>
+    simp [typeOf, typeOfVar, ok] at h₃
+    split at h₃ <;>
+    (
+      simp at h₃
+      rcases h₃ with ⟨h₃, _⟩
+      subst h₃
+      simp only [TypedExpr.toExpr]
+    )
+  case _ c₁ env x₁ x₂ x₃ hᵢ₁ hᵢ₂ hᵢ₃ =>
+    simp [typeOf] at h₃
+    generalize h₁ᵢ : typeOf x₁ c₁ env = res₁
+    cases res₁
+    case ok ty =>
+      simp [h₁ᵢ] at h₃
+      simp [typeOfIf, ok] at h₃
+      specialize hᵢ₁ h₁ h₂ h₁ᵢ
+      split at h₃
+      case _ heq =>
+        simp [do_ok_eq_ok] at h₃
+        rcases h₃ with ⟨_, _, h₃₁, h₃₂, h₃₃⟩
+        subst h₃₂
+        simp only [evaluate, TypedExpr.toExpr, ←hᵢ₁]
+        generalize h₃ : evaluate x₁ request entities = res₁
+        cases res₁
+        case _ => simp only [Result.as, Except.bind_err, ite_self]
+        case _ =>
+          have h₄ := type_of_is_sound h₁ h₂ h₁ᵢ
+          rcases h₄ with ⟨h₄₁, _, h₄₂, h₄₃⟩
+          rw [heq] at h₄₃
+          replace h₄₃ := instance_of_tt_is_true h₄₃
+          subst h₄₃
+          simp [EvaluatesTo, h₃] at h₄₂
+          subst h₄₂
+          simp [Result.as, Coe.coe, Value.asBool]
+          simp [GuardedCapabilitiesInvariant] at h₄₁
+          specialize h₄₁ h₃
+          exact hᵢ₂ _ (capability_union_invariant h₁ h₄₁) h₂ h₃₁
+      case _ heq =>
+        simp [do_ok_eq_ok] at h₃
+        rcases h₃ with ⟨_, h₃₁, h₃₂⟩
+        subst h₃₂
+        simp only [evaluate, TypedExpr.toExpr, ←hᵢ₁]
+        generalize h₃ : evaluate x₁ request entities = res₁
+        cases res₁
+        case _ => simp only [Result.as, Except.bind_err, ite_self]
+        case _ =>
+          have h₄ := type_of_is_sound h₁ h₂ h₁ᵢ
+          rcases h₄ with ⟨h₄₁, _, h₄₂, h₄₃⟩
+          rw [heq] at h₄₃
+          replace h₄₃ := instance_of_ff_is_false h₄₃
+          subst h₄₃
+          simp [EvaluatesTo, h₃] at h₄₂
+          subst h₄₂
+          simp [Result.as, Coe.coe, Value.asBool]
+          exact hᵢ₃ h₁ h₂ h₃₁
+      case _ heq =>
+        simp [do_eq_ok] at h₃
+        rcases h₃ with ⟨_, _, h₃₁, _, _, h₃₂, h₃₃⟩
+        split at h₃₃ <;> simp [err] at h₃₃
+        rcases h₃₃ with ⟨h₃₃, _⟩
+        subst h₃₃
+        simp [TypedExpr.toExpr, evaluate, ←hᵢ₁]
+        generalize h₃ : evaluate x₁ request entities = res₁
+        cases res₁
+        case _ => simp only [Result.as, Except.bind_err, ite_self]
+        case _ =>
+          have h₄ := type_of_is_sound h₁ h₂ h₁ᵢ
+          rcases h₄ with ⟨h₄₁, _, h₄₂, h₄₃⟩
+          rw [heq] at h₄₃
+          rcases instance_of_anyBool_is_bool h₄₃ with ⟨b₁, h₄₃⟩
+          subst h₄₃
+          simp [EvaluatesTo, h₃] at h₄₂
+          subst h₄₂
+          simp [Result.as, Coe.coe, Value.asBool]
+          cases b₁
+          case _ =>
+            simp only [Bool.false_eq_true, ↓reduceIte]
+            exact hᵢ₃ h₁ h₂ h₃₂
+          case _ =>
+            simp only [↓reduceIte]
+            simp [GuardedCapabilitiesInvariant] at h₄₁
+            specialize h₄₁ h₃
+            exact hᵢ₂ _ (capability_union_invariant h₁ h₄₁) h₂ h₃₁
+      case _ => simp only [err, reduceCtorEq] at h₃
+    case error => simp only [h₁ᵢ, Except.bind_err, reduceCtorEq] at h₃
+  case _ c₁ env x₁ x₂ hᵢ₁ hᵢ₂ =>
+    simp [typeOf, do_eq_ok] at h₃
+    rcases h₃ with ⟨_, _, h₃₁, h₃₂⟩
+    specialize hᵢ₁ h₁ h₂ h₃₁
+    simp [typeOfAnd] at h₃₂
+    split at h₃₂ <;> simp [ok, err] at h₃₂
+    case _ heq =>
+      rcases h₃₂ with ⟨h₃₂, _⟩
+      subst h₃₂
+      simp [evaluate, ←hᵢ₁]
+      generalize h₃ : evaluate x₁ request entities = res₁
+      cases res₁
+      case _ => simp only [Result.as, Except.bind_err]
+      case _ =>
+        have h₄ := type_of_is_sound h₁ h₂ h₃₁
+        rcases h₄ with ⟨_, _, h₄₁, h₄₂⟩
+        rw [heq] at h₄₂
+        replace h₄₂ := instance_of_ff_is_false h₄₂
+        subst h₄₂
+        simp only [EvaluatesTo, h₃, reduceCtorEq, Except.ok.injEq, false_or] at h₄₁
+        subst h₄₁
+        simp only [Result.as, Coe.coe, Value.asBool, Except.bind_ok, ↓reduceIte]
+    case _ heq =>
+      simp [do_eq_ok] at h₃₂
+      rcases h₃₂ with ⟨_, _, h₃₂₁, h₃₂₂⟩
+      split at h₃₂₂ <;> simp [err] at h₃₂₂
+      all_goals
+        rcases h₃₂₂ with ⟨h₃₂₂, _⟩
+        subst h₃₂₂
+        have h₄ := type_of_is_sound h₁ h₂ h₃₁
+        rcases h₄ with ⟨h₄₁, _, h₄₂, h₄₃⟩
+        simp [TypedExpr.toExpr, evaluate, ←hᵢ₁]
+        generalize h₃ : evaluate x₁ request entities = res₁
+        cases res₁
+        case _ => simp only [Result.as, Except.bind_err]
+        case _ =>
+          rw [heq] at h₄₃
+          rcases instance_of_bool_is_bool h₄₃ with ⟨b₁, h₄₃⟩
+          simp [EvaluatesTo, h₃] at h₄₂
+          subst h₄₂
+          subst h₄₃
+          cases b₁
+          case _ =>
+            simp only [Result.as, Coe.coe, Value.asBool, Except.bind_ok, ↓reduceIte]
+          case _ =>
+            simp [Result.as, Coe.coe, Value.asBool]
+            simp [GuardedCapabilitiesInvariant] at h₄₁
+            specialize h₄₁ h₃
+            specialize hᵢ₂ _ (capability_union_invariant h₁ h₄₁) h₂ h₃₂₁
+            simp only [hᵢ₂]
+  case _ c₁ env x₁ x₂ hᵢ₁ hᵢ₂ =>
+    simp [typeOf, do_eq_ok] at h₃
+    rcases h₃ with ⟨_, _, h₃₁, h₃₂⟩
+    simp [typeOfOr] at h₃₂
+    specialize hᵢ₁ h₁ h₂ h₃₁
+    split at h₃₂ <;> simp [ok, err] at h₃₂
+    case _ heq =>
+      rcases h₃₂ with ⟨h₃₂, _⟩
+      subst h₃₂
+      simp [evaluate, ←hᵢ₁]
+      generalize h₃ : evaluate x₁ request entities = res₁
+      cases res₁
+      case _ => simp [Result.as, Except.bind_err]
+      case _ =>
+        have h₄ := type_of_is_sound h₁ h₂ h₃₁
+        rcases h₄ with ⟨_, _, h₄₁, h₄₂⟩
+        rw [heq] at h₄₂
+        replace h₄₂ := instance_of_tt_is_true h₄₂
+        subst h₄₂
+        simp only [EvaluatesTo, h₃, reduceCtorEq, Except.ok.injEq, false_or] at h₄₁
+        subst h₄₁
+        simp only [Result.as, Coe.coe, Value.asBool, Except.bind_ok, ↓reduceIte]
+    case _ heq =>
+      simp [do_eq_ok] at h₃₂
+      rcases h₃₂ with ⟨_, _, h₃₂₁, h₃₂₂⟩
+      specialize hᵢ₂ h₁ h₂ h₃₂₁
+      split at h₃₂₂ <;> simp [err] at h₃₂₂
+      rcases h₃₂₂ with ⟨h₃₂₂, _⟩
+      subst h₃₂₂
+      simp only [evaluate, hᵢ₁, hᵢ₂, bind_pure_comp, TypedExpr.toExpr]
+    case _ heq =>
+      simp [do_eq_ok] at h₃₂
+      rcases h₃₂ with ⟨_, _, h₃₂₁, h₃₂₂⟩
+      specialize hᵢ₂ h₁ h₂ h₃₂₁
+      split at h₃₂₂ <;> simp [err] at h₃₂₂
+      all_goals
+        rcases h₃₂₂ with ⟨h₃₂₂, _⟩
+        subst h₃₂₂
+        have h₄ := type_of_is_sound h₁ h₂ h₃₁
+        rcases h₄ with ⟨h₄₁, _, h₄₂, h₄₃⟩
+        simp [TypedExpr.toExpr, evaluate, ←hᵢ₁]
+        generalize h₃ : evaluate x₁ request entities = res₁
+        cases res₁
+        case _ => simp only [Result.as, Except.bind_err]
+        case _ =>
+          rw [heq] at h₄₃
+          rcases instance_of_bool_is_bool h₄₃ with ⟨b₁, h₄₃⟩
+          simp [EvaluatesTo, h₃] at h₄₂
+          subst h₄₂
+          subst h₄₃
+          cases b₁
+          case _ =>
+            simp only [Result.as, Coe.coe, Value.asBool, hᵢ₂, Except.bind_ok, Bool.false_eq_true,
+              ↓reduceIte]
+          case _ =>
+            simp only [Result.as, Coe.coe, Value.asBool, Except.bind_ok, ↓reduceIte]
+  case _ hᵢ =>
+    simp [typeOf, do_eq_ok] at h₃
+    rcases h₃ with ⟨_, ⟨_, h₃₁⟩, h₃₂⟩
+    simp [typeOfUnaryApp] at h₃₂
+    specialize hᵢ h₁ h₂ h₃₁
+    split at h₃₂ <;>
+    simp [ok, err] at h₃₂ <;>
+    try (
+      rcases h₃₂ with ⟨h₃₂, _⟩
+      subst h₃₂
+      simp only [TypedExpr.toExpr, evaluate, hᵢ]
+    )
+  case _ hᵢ₁ hᵢ₂ =>
+    simp [typeOf, do_eq_ok] at h₃
+    rcases h₃ with ⟨_, ⟨_, h₃₁⟩, _, ⟨_, h₃₂⟩, h₃₃⟩
+    specialize hᵢ₁ h₁ h₂ h₃₁
+    specialize hᵢ₂ h₁ h₂ h₃₂
+    simp [typeOfBinaryApp] at h₃₃
+    split at h₃₃ <;> try simp [ok, err] at h₃₃
+    any_goals
+      rcases h₃₃ with ⟨h₃₃, _⟩
+      subst h₃₃
+      simp only [TypedExpr.toExpr, evaluate, hᵢ₁, hᵢ₂]
+    any_goals
+      simp [do_ok_eq_ok] at h₃₃
+      rcases h₃₃ with ⟨_, h₃₃₁, h₃₃₂⟩
+      subst h₃₃₂
+      simp only [TypedExpr.toExpr, evaluate, hᵢ₁, hᵢ₂]
+    case _ =>
+      simp [typeOfEq] at h₃₃
+      split at h₃₃ <;>
+      split at h₃₃ <;>
+      try (
+        simp [ok] at h₃₃
+        rcases h₃₃ with ⟨h₃₃, _⟩
+        subst h₃₃
+        try simp [evaluate] at hᵢ₁
+        try simp [evaluate] at hᵢ₂
+        simp only [TypedExpr.toExpr, evaluate, hᵢ₁, hᵢ₂]
+      )
+      split at h₃₃ <;> simp [ok, err] at h₃₃
+      rcases h₃₃ with ⟨h₃₃, _⟩
+      subst h₃₃
+      simp only [TypedExpr.toExpr, evaluate, hᵢ₁, hᵢ₂]
+  case _ hᵢ =>
+    simp only [typeOf, do_eq_ok, Prod.exists, exists_and_right] at h₃
+    rcases h₃ with ⟨ty, ⟨c, h₃₁⟩, h₃₂⟩
+    simp only [typeOfHasAttr, List.empty_eq] at h₃₂
+    specialize hᵢ h₁ h₂ h₃₁
+    split at h₃₂
+    case _ =>
+      simp only [ok, do_ok_eq_ok, Prod.mk.injEq, Prod.exists, exists_eq_right_right] at h₃₂
+      rcases h₃₂ with ⟨_, _, h₃₂⟩
+      subst h₃₂
+      simp only [TypedExpr.toExpr, evaluate, hᵢ]
+    case _ =>
+      split at h₃₂ <;>
+      try split at h₃₂
+      case _ =>
+        simp only [ok, do_ok_eq_ok, Prod.mk.injEq, Prod.exists, exists_eq_right_right] at h₃₂
+        rcases h₃₂ with ⟨_, _, h₃₂⟩
+        subst h₃₂
+        simp only [TypedExpr.toExpr, evaluate, hᵢ]
+      case _ =>
+        simp only [ok, Except.ok.injEq, Prod.mk.injEq, List.nil_eq] at h₃₂
+        rcases h₃₂ with ⟨h₃₂, _⟩
+        subst h₃₂
+        simp only [TypedExpr.toExpr, evaluate, hᵢ]
+      simp only [err, reduceCtorEq] at h₃₂
+    simp only [err, reduceCtorEq] at h₃₂
+  case _ hᵢ =>
+    simp only [typeOf, do_eq_ok, Prod.exists, exists_and_right] at h₃
+    rcases h₃ with ⟨ty, ⟨c, h₃₁⟩, h₃₂⟩
+    simp only [typeOfGetAttr, List.empty_eq] at h₃₂
+    specialize hᵢ h₁ h₂ h₃₁
+    split at h₃₂
+    case _ =>
+      simp only [ok, do_ok_eq_ok, Prod.mk.injEq, Prod.exists, exists_eq_right_right] at h₃₂
+      rcases h₃₂ with ⟨_, _, h₃₂⟩
+      subst h₃₂
+      simp only [TypedExpr.toExpr, evaluate, hᵢ]
+    case _ =>
+      split at h₃₂
+      simp only [ok, do_ok_eq_ok, Prod.mk.injEq, Prod.exists, exists_eq_right_right] at h₃₂
+      rcases h₃₂ with ⟨_, _, h₃₂⟩
+      subst h₃₂
+      simp only [TypedExpr.toExpr, evaluate, hᵢ]
+      simp only [err, reduceCtorEq] at h₃₂
+    simp only [err, reduceCtorEq] at h₃₂
+  case _ c₁ env xs hᵢ =>
+    simp only [typeOf, do_eq_ok, Prod.exists, exists_and_right] at h₃
+    rcases h₃ with ⟨ty, h₃₁, h₃₂⟩
+    simp [List.mapM₁_eq_mapM (fun x => justType (typeOf x c₁ env)), List.mapM_ok_iff_forall₂] at h₃₁
+    simp [typeOfSet] at h₃₂
+    split at h₃₂ <;> simp [err] at h₃₂
+    split at h₃₂ <;> simp [ok] at h₃₂
+    rcases h₃₂ with ⟨h₃₂, _⟩
+    subst h₃₂
+    simp only [TypedExpr.toExpr, evaluate, List.map₁_eq_map, List.mapM₁_eq_mapM (fun x => evaluate x request entities), List.mapM_map]
+    have h₄ := type_of_ok_list h₃₁ (λ x₁ h => hᵢ x₁ h h₁ h₂)
+    simp only [List.forall₂_implies_mapM_eq _ _ h₄, List.mapM_cons, bind_pure_comp, bind_assoc,
+      bind_map_left]
+  case _ c₁ env axs hᵢ =>
+    simp [typeOf, do_eq_ok] at h₃
+    rcases h₃ with ⟨atys, h₃₁, h₃₂⟩
+    simp [ok] at h₃₂
+    rcases h₃₂ with ⟨h₃₂, _⟩
+    subst h₃₂
+    simp [evaluate, List.mapM₂, List.attach₂]
+    rw [List.mapM_pmap_subtype (fun (x : Attr × Expr) => bindAttr x.fst (evaluate x.snd request entities))]
+    simp [TypedExpr.toExpr, List.attach₂]
+    rw [List.map_pmap_subtype (fun (x : Attr × TypedExpr) => (x.fst, x.snd.toExpr))]
+    simp [evaluate, List.mapM₂, List.attach₂]
+    rw [List.mapM_pmap_subtype (fun (x : Attr × Expr) => bindAttr x.fst (evaluate x.snd request entities))]
+    simp [List.mapM_map]
+    simp [evaluate, List.mapM₂, List.attach₂] at h₃₁
+    rw [List.mapM_pmap_subtype (fun (x : Attr × Expr) => Except.map (fun x_1 => (x.fst, x_1.fst)) (typeOf x.snd c₁ env)), List.mapM_ok_iff_forall₂] at h₃₁
+    have h₄ := type_of_ok_attr_list h₃₁ (λ a₁ x₁ h => hᵢ a₁ x₁ h h₁ h₂)
+    simp only [List.forall₂_implies_mapM_eq _ _ h₄]
+  case _ c₁ env xfn xs hᵢ =>
+    simp [typeOf, do_eq_ok] at h₃
+    rcases h₃ with ⟨tys, h₃₁, h₃₂⟩
+    simp [List.mapM₁_eq_mapM fun x => justType (typeOf x c₁ env), List.mapM_ok_iff_forall₂] at h₃₁
+    have h₄ := type_of_ok_list h₃₁ (λ x₁ h => hᵢ x₁ h h₁ h₂)
+    exact type_of_preserves_evaluation_results_call h₃₂ (List.forall₂_implies_mapM_eq _ _ h₄)
